add mgs

programs/GramSchmidt.fst
@@ -6,59 +6,70 @@ noeq type rect : pos -> pos -> Type =
   | Rect1 : #n:pos -> cvec n -> rect n 1
   | RectK : #n:pos -> #k:pos -> rect n k -> cvec n -> rect n (k + 1)
 
-assume val nnz_vec (#n:pos) (#o:orient) (v:vec o n) : prop
+assume val nnz_vec  (#n:pos) (#o:orient) (v:vec o n) : prop
 assume val unit_vec (#n:pos) (#o:orient) (v:vec o n) : prop
-assume val unit_vec_nnz (#n:pos) (#o:orient) (v:vec o n) : 
+
+assume val unit_vec_nnz (#n:pos) (#o:orient) (v:vec o n) :
     Lemma (requires unit_vec v) (ensures nnz_vec v) [SMTPat (nnz_vec v)]
 
+(* v is linearly independent of the columns of m *)
 assume val mat_vec_ind (#n:pos) (#k:pos) (m:rect n k) (v:cvec n) : prop
+(* v is orthogonal to every column of m *)
 assume val mat_vec_ortho (#n:pos) (#k:pos) (m:rect n k) (v:cvec n) : prop
-assume val ortho_is_ind (#n:pos) (#k:pos) (m:rect n k) (v:cvec n) : 
-  Lemma (requires mat_vec_ortho m v) (ensures mat_vec_ind m v) [SMTPat (mat_vec_ortho m v)]
 
+assume val ortho_nnz (#n:pos) (#k:pos) (m:rect n k) (v:cvec n) :
+    Lemma (requires mat_vec_ortho m v) (ensures nnz_vec v) [SMTPat (mat_vec_ortho m v)]
+assume val ortho_is_ind (#n:pos) (#k:pos) (m:rect n k) (v:cvec n) :
+    Lemma (requires mat_vec_ortho m v) (ensures mat_vec_ind m v) [SMTPat (mat_vec_ortho m v)]
+
+(* entire matrix has lin ind/ortho cols *)
 let rec linind (#n:pos) (#k:pos) (m:rect n k) : prop = 
   match m with 
   | Rect1 v -> nnz_vec v 
-  | RectK m' v -> linind m' /\ mat_vec_ind m' v
+  | RectK m' v -> linind m' /\ mat_vec_ind m' v /\ nnz_vec v
 
 let rec ortho (#n:pos) (#k:pos) (m:rect n k) : prop = 
   match m with 
   | Rect1 v -> unit_vec v
-  | RectK m' v -> ortho m' /\ mat_vec_ortho m' v
+  | RectK m' v -> ortho m' /\ mat_vec_ortho m' v /\ unit_vec v
 
 let same_col_span (#n:pos) (#k:pos) (m1 m2:rect n k) : prop =
-  forall (v:cvec n). (mat_vec_ind m1 v <==> mat_vec_ind m2 v) /\ 
-    (mat_vec_ortho m1 v <==> mat_vec_ortho m2 v)
+  forall (v:cvec n). mat_vec_ind m1 v <==> mat_vec_ind m2 v
 
-let same_vec_span (#n:pos) (v1 v2:cvec n) : prop =
-  forall (#k:pos) (m:rect n k). (mat_vec_ind m v1 <==> mat_vec_ind m v2) /\
-    (mat_vec_ortho m v1 <==> mat_vec_ortho m v2)
+assume val span_pres_ortho (#n:pos) (#k:pos) (m1 m2:rect n k) :
+    Lemma (requires same_col_span m1 m2)
+          (ensures forall (v:cvec n). mat_vec_ortho m1 v <==> mat_vec_ortho m2 v)
+          [SMTPat (same_col_span m1 m2)]
 
-assume val vec_mat1_span (#n:pos) (v1 v2:cvec n) : 
-  Lemma (requires same_vec_span v1 v2) (ensures same_col_span (Rect1 v1) (Rect1 v2))
-  [SMTPat (same_vec_span v1 v2)]
+(* can append a column *)
+assume val vec_span_cong (#n:pos) (v1 v2:cvec n) :
+    Lemma (requires same_col_span (Rect1 v1) (Rect1 v2))
+          (ensures forall (#k:pos) (m:rect n k).
+                     same_col_span (RectK m v1) (RectK m v2) /\
+                     (mat_vec_ortho m v1 <==> mat_vec_ortho m v2) /\
+                     (mat_vec_ind m v1 <==> mat_vec_ind m v2))
+          [SMTPat (same_col_span (Rect1 v1) (Rect1 v2))]
 
-assume val vec_pres_span (#n:pos) (v1 v2:cvec n) : 
-  Lemma (requires same_vec_span v1 v2) (ensures forall (#k:pos) (m:rect n k). same_col_span (RectK m v1) (RectK m v2))
-  [SMTPat (same_vec_span v1 v2)]
+assume val mat_span_cong (#n:pos) (#k:pos) (m1 m2:rect n k) :
+    Lemma (requires same_col_span m1 m2)
+          (ensures forall (v:cvec n).
+                     same_col_span (RectK m1 v) (RectK m2 v))
+          [SMTPat (same_col_span m1 m2)]
 
-assume val mat_pres_span (#n:pos) (#k:pos) (m1 m2:rect n k) : 
-  Lemma (requires same_col_span m1 m2) (ensures forall (v:cvec n). same_col_span (RectK m1 v) (RectK m2 v))
-  [SMTPat (same_col_span m1 m2)]
+(* operations *)
+assume val normalize (#n:pos) (v1:cvec n{nnz_vec v1}) : (v2:cvec n{unit_vec v2})
 
-assume val normalize (#n:pos) (v1:cvec n{nnz_vec v1}) : 
-  (v2:cvec n{unit_vec v2})
-
-assume val normalize_pres_span (#n:pos) (v:cvec n{nnz_vec v})
-  : Lemma (same_vec_span v (normalize v))
+assume val normalize_pres_span (#n:pos) (v:cvec n{nnz_vec v}) :
+    Lemma (same_col_span (Rect1 v) (Rect1 (normalize v)))
           [SMTPat (normalize v)]
 
-assume val residual (#n:pos) (#k:pos) (m:rect n k) 
-  (v1:cvec n{mat_vec_ind m v1}) : v2:cvec n{nnz_vec v2 /\ mat_vec_ortho m v2}
+assume val residual (#n:pos) (#k:pos) (m:rect n k)
+    (v1:cvec n{mat_vec_ind m v1}) : v2:cvec n{mat_vec_ortho m v2 /\ same_col_span (RectK m v1) (RectK m v2)}
 
-assume val residual_pres_span (#n:pos) (#k:pos) (m:rect n k) (v:cvec n{mat_vec_ind m v}) : 
-  Lemma (same_col_span (RectK m v) (RectK m (residual m v))) [SMTPat (residual m v)]
+assume val residual_mat (#n:pos) (#k:pos) (v:cvec n{unit_vec v}) (m1:rect n k) : 
+  m2:rect n k{mat_vec_ortho m2 v /\ linind m2 /\ same_col_span (RectK m1 v) (RectK m2 v)}
 
+(* regular gram schmidt *)
 let rec gramschmidt (#n:pos) (#k:pos) (m:rect n k{linind m}) : 
   (q:rect n k{ortho q /\ same_col_span m q}) = 
   match m with 
@@ -78,3 +89,14 @@ let rec gramschmidt (#n:pos) (#k:pos) (m:rect n k{linind m}) :
     // assert mat_vec_ortho q' res;
     // assert mat_vec_ortho q' q;
     r
+
+(* modified gram schmidt *)
+let rec mgs (#n:pos) (#k:pos) (m:rect n k{linind m}) : 
+  (q:rect n k{ortho q /\ same_col_span m q}) = 
+  match m with 
+  | Rect1 v -> Rect1 (normalize v)
+  | RectK m' v -> 
+    let q1 = normalize v in
+    let m'' = residual_mat q1 m' in 
+    let q = mgs m'' in 
+    RectK q q1
